rupicola/SyntacticTypes.fst
@@ -11,11 +11,11 @@ open STLC
 type typ =
   | TUnit : typ
   | TArr  : typ -> typ -> typ
-  
+
 (** We have to very careful on how we define this elaboration of types.
     We'll face universe problems when using monads `Type u#a -> Type u#(max 1 a)`.
     See also: https://fstar.zulipchat.com/#narrow/stream/214975-fstar-ml-interop/topic/Language.20characterization **)
-let rec elab_typ (t:typ) : Type0 = 
+let rec elab_typ (t:typ) : Type0 =
   match t with
   | TUnit -> unit
   | TArr t1 t2 -> (elab_typ t1 -> elab_typ t2)
@@ -33,3 +33,9 @@ let extend (t:typ) (g:env)
 
 let fv_in_env (g:env) (e:exp) : Type0 =
   forall (fv:var). fv `memP` free_vars e ==> Some? (g fv)
+
+let lem_no_fv_is_closed (e:exp) : Lemma
+  (requires fv_in_env empty e)
+  (ensures is_closed e)
+  [SMTPat (is_closed e)] =
+  ()
